\begin{align}
I_{6}
&=\int_{0}^{1}\frac{\ln{(t+1)}\ln{(2t+1)}}{2t+1}\,\mathrm{d}t\\
&=\left[\frac14\ln{(t+1)}\ln^2{(2t+1)}\right]_{0}^{1}-\frac14\int_{0}^{1}\frac{\ln^2{(2t+1)}}{t+1}\,\mathrm{d}t\\
&=\frac14\ln{2}\ln^2{3}-\frac14\int_{0}^{1}\frac{\ln^2{(2t+1)}}{t+1}\,\mathrm{d}t\\
&=\frac14\ln{2}\ln^2{3}-\frac14\int_{1}^{3}\frac{\ln^2{u}}{u+1}\,\mathrm{d}u\\
&=\frac14\ln{2}\ln^2{3}-\frac14\left[\ln^2{u}\ln{(u+1)}\right]_{1}^{3}+\frac14\int_{1}^{3}\frac{2\ln{u}\ln{(u+1)}}{u}\,\mathrm{d}u\\
&=\frac14\ln{2}\ln^2{3}-\frac12\ln{2}\ln^2{3}+\frac12\int_{1}^{3}\frac{\ln{u}\ln{(u+1)}}{u}\,\mathrm{d}u\\
&=-\frac14\ln{2}\ln^2{3}-\frac12\left[\ln{u}\operatorname{Li}_2{\left(-u\right)}\right]_{1}^{3}+\frac12\int_{1}^{3}\frac{\operatorname{Li}_2{\left(-u\right)}}{u}\,\mathrm{d}u\\
&=-\frac14\ln{2}\ln^2{3}-\frac12\ln{3}\operatorname{Li}_2{\left(-3\right)}+\frac12\int_{1}^{3}\frac{\operatorname{Li}_2{\left(-u\right)}}{u}\,\mathrm{d}u\\
&=-\frac14\ln{2}\ln^2{3}-\frac12\ln{3}\operatorname{Li}_2{\left(-3\right)}+\frac12\left[\operatorname{Li}_3{\left(-u\right)}\right]_{1}^{3}\\
&=-\frac14\ln{2}\ln^2{3}-\frac12\ln{3}\operatorname{Li}_2{\left(-3\right)}+\frac12\operatorname{Li}_3{\left(-3\right)}-\frac12\operatorname{Li}_3{\left(-1\right)}\\
&=-\frac14\ln{2}\ln^2{3}+\frac12\ln{3}\operatorname{Li}_2{\left(\frac34\right)} -\frac12\operatorname{Li}_3{\left(\frac{3}{4}\right)}-\frac12\operatorname{Li}_3{\left(\frac{1}{4}\right)}+\frac43\ln^3{(2)}-\frac{\pi^2}{6}\ln{(2)}+\frac78\zeta{(3)}.
\end{align}