\sum_{r=1}^\infty\frac{2r-1}{r(r+1)(r+2)} = \sum_{r=1}^\infty\frac{1}{2r}-\frac{1}{r+1}+\frac{1}{2(r+2)} \\ = \frac{1}{2}\sum_{r=1}^\infty \frac{1}{r}-\sum_{r=1}^\infty\frac{1}{r+1}+\frac{1}{2}\sum_{r=1}^\infty\frac{1}{(r+2)} \\ = \frac{1}{2}\left(1+\frac{1}{2}+\sum_{r=3}^\infty \frac{1}{r}\right)-\left(\frac{1}{2}+\sum_{r=3}^\infty\frac{1}{r}\right)+\frac{1}{2}\sum_{r=3}^\infty\frac{1}{r} \\ = \frac{1}{2}\left(1+\frac{1}{2}\right)-\frac{1}{2}+\sum_{r=3}^\infty \frac{1}{r}\left(\frac{1}{2}-1+\frac{1}{2} \right)